Weidenbach_Book/IsaSAT_Lookup_Conflict.thy
@@ -629,17 +629,15 @@ sepref_thm resolve_lookup_conflict_merge_code
   supply length_rll_def[simp] nth_rll_def[simp] uint_max_def[simp]
     uint32_nat_assn_one[sepref_fr_rules] image_image[simp] literals_are_in_\<L>\<^sub>i\<^sub>n_in_\<L>\<^sub>a\<^sub>l\<^sub>l[simp]
     literals_are_in_\<L>\<^sub>i\<^sub>n_trail_get_level_uint_max[dest]
-    Suc_uint32_nat_assn_hnr[sepref_fr_rules]
+    Suc_uint32_nat_assn_hnr[sepref_fr_rules] fmap_length_rll_u_def[simp]
   unfolding resolve_lookup_conflict_aa_def lookup_conflict_merge_def add_to_lookup_conflict_def
-    PR_CONST_def nth_rll_def[symmetric] length_rll_def[symmetric]
-    length_aa_u_def[symmetric] outlearned_add_def clvls_add_def
+    PR_CONST_def nth_rll_def[symmetric]
+    outlearned_add_def clvls_add_def
+    isasat_codegen
+    fmap_rll_u_def[symmetric]
+    fmap_rll_def[symmetric]
   apply (rewrite at \<open>_ + \<hole>\<close> annotate_assn[where A = \<open>uint32_nat_assn\<close>])
   supply [[goals_limit = 1]]
-    apply sepref_dbg_keep
-      apply sepref_dbg_trans_keep
-           apply sepref_dbg_trans_step_keep
-           apply sepref_dbg_side_unfold apply (auto simp: )[]
-
   by sepref
 
 concrete_definition (in -) resolve_lookup_conflict_merge_code
@@ -654,20 +652,23 @@ lemmas resolve_lookup_conflict_aa_hnr[sepref_fr_rules] =
 sepref_register set_lookup_conflict_aa
 sepref_thm set_lookup_conflict_aa_code
   is \<open>uncurry6 (PR_CONST set_lookup_conflict_aa)\<close>
-  :: \<open>[\<lambda>((((((M, N), i), (_, xs)), _), _), _). i < length N \<and> literals_are_in_\<L>\<^sub>i\<^sub>n_trail M \<and>
-        (\<forall>j<length (N!i). atm_of (N!i!j) < length (snd xs)) \<and> no_dup M \<and>
-        literals_are_in_\<L>\<^sub>i\<^sub>n (mset (N!i)) \<and>
-        length (N!i) \<le> uint_max]\<^sub>a
+  :: \<open>[\<lambda>((((((M, N), i), (_, xs)), _), _), _). i \<in># dom_m N \<and> literals_are_in_\<L>\<^sub>i\<^sub>n_trail M \<and>
+        (\<forall>j<length (N\<propto>i). atm_of (N\<propto>i!j) < length (snd xs)) \<and> no_dup M \<and>
+        literals_are_in_\<L>\<^sub>i\<^sub>n (mset (N\<propto>i)) \<and>
+        length (N\<propto>i) \<le> uint_max]\<^sub>a
       trail_assn\<^sup>k *\<^sub>a clauses_ll_assn\<^sup>k *\<^sub>a nat_assn\<^sup>k *\<^sub>a conflict_option_rel_assn\<^sup>d *\<^sub>a
          uint32_nat_assn\<^sup>k *\<^sub>a lbd_assn\<^sup>d  *\<^sub>a out_learned_assn\<^sup>d \<rightarrow>
       conflict_option_rel_assn *a uint32_nat_assn *a lbd_assn *a out_learned_assn\<close>
   supply length_rll_def[simp] nth_rll_def[simp] uint_max_def[simp]
     uint32_nat_assn_one[sepref_fr_rules] image_image[simp] literals_are_in_\<L>\<^sub>i\<^sub>n_in_\<L>\<^sub>a\<^sub>l\<^sub>l[simp]
     literals_are_in_\<L>\<^sub>i\<^sub>n_trail_get_level_uint_max[dest]
-    Suc_uint32_nat_assn_hnr[sepref_fr_rules]
+    Suc_uint32_nat_assn_hnr[sepref_fr_rules]  fmap_length_rll_u_def[simp]
   unfolding set_lookup_conflict_aa_def lookup_conflict_merge_def add_to_lookup_conflict_def
     PR_CONST_def nth_rll_def[symmetric] length_rll_def[symmetric]
     length_aa_u_def[symmetric] outlearned_add_def clvls_add_def
+    isasat_codegen
+    fmap_rll_u_def[symmetric]
+    fmap_rll_def[symmetric]
   apply (rewrite at \<open>_ + \<hole>\<close> annotate_assn[where A = \<open>uint32_nat_assn\<close>])
   supply [[goals_limit = 1]]
   by sepref
@@ -1051,10 +1052,10 @@ qed
 
 lemma resolve_lookup_conflict_aa_set_conflict:
   \<open>(uncurry6 set_lookup_conflict_aa, uncurry6 set_conflict_m) \<in>
-    [\<lambda>((((((M, N), i), xs), clvls), lbd), outl). i < length N \<and> xs = None \<and> distinct (N ! i) \<and>
-       literals_are_in_\<L>\<^sub>i\<^sub>n (mset (N ! i)) \<and> \<not>tautology (mset (N ! i)) \<and> clvls = 0 \<and>
+    [\<lambda>((((((M, N), i), xs), clvls), lbd), outl). i \<in># dom_m N \<and> xs = None \<and> distinct (N \<propto> i) \<and>
+       literals_are_in_\<L>\<^sub>i\<^sub>n (mset (N \<propto> i)) \<and> \<not>tautology (mset (N \<propto> i)) \<and> clvls = 0 \<and>
        out_learned M None outl]\<^sub>f
-    \<langle>Id\<rangle>list_rel \<times>\<^sub>f \<langle>\<langle>Id\<rangle>list_rel\<rangle>list_rel \<times>\<^sub>f nat_rel \<times>\<^sub>f option_lookup_clause_rel \<times>\<^sub>f nat_rel \<times>\<^sub>f Id
+    \<langle>Id\<rangle>list_rel \<times>\<^sub>f Id \<times>\<^sub>f nat_rel \<times>\<^sub>f option_lookup_clause_rel \<times>\<^sub>f nat_rel \<times>\<^sub>f Id
          \<times>\<^sub>f Id  \<rightarrow>
       \<langle>option_lookup_clause_rel \<times>\<^sub>r nat_rel \<times>\<^sub>r Id \<times>\<^sub>r Id \<rangle>nres_rel\<close>
 proof -
@@ -1062,11 +1063,11 @@ proof -
     \<le> \<Down> (option_lookup_clause_rel \<times>\<^sub>r Id)
        (set_conflict_m M N i None clvls lbd outl)\<close>
     if
-      \<open>i < length N\<close> and
+      \<open>i \<in># dom_m N\<close> and
       ocr: \<open>((b, n, xs), None) \<in> option_lookup_clause_rel\<close> and
-     dist: \<open>distinct (N! i)\<close> and
-     lits: \<open>literals_are_in_\<L>\<^sub>i\<^sub>n (mset (N ! i))\<close> and
-     tauto: \<open>\<not>tautology (mset (N ! i))\<close> and
+     dist: \<open>distinct (N \<propto> i)\<close> and
+     lits: \<open>literals_are_in_\<L>\<^sub>i\<^sub>n (mset (N \<propto> i))\<close> and
+     tauto: \<open>\<not>tautology (mset (N \<propto> i))\<close> and
      \<open>clvls = 0\<close> and
      out: \<open>out_learned M None outl\<close>
     for b n xs N i M clvls lbd outl
@@ -1080,7 +1081,7 @@ proof -
     have T: \<open>((False, n, xs), Some {#}) \<in> option_lookup_clause_rel\<close>
       using ocr unfolding option_lookup_clause_rel_def by auto
     show ?thesis unfolding set_lookup_conflict_aa_def set_conflict_m_def
-      using lookup_conflict_merge'_spec[of False n xs \<open>{#}\<close> \<open>N!i\<close> 0 _ 0 outl lbd] that dist T
+      using lookup_conflict_merge'_spec[of False n xs \<open>{#}\<close> \<open>N\<propto>i\<close> 0 _ 0 outl lbd] that dist T
       by (auto simp: lookup_conflict_merge_normalise uint_max_def merge_conflict_m_g_def)
   qed
   show ?thesis
@@ -1090,8 +1091,8 @@ qed
 
 theorem resolve_lookup_conflict_merge_code_set_conflict[sepref_fr_rules]:
   \<open>(uncurry6 set_lookup_conflict_aa_code, uncurry6 set_conflict_m) \<in>
-  [\<lambda>((((((M, N), i), xs), clvls), lbd), outl). clvls = 0 \<and> i < length N \<and> xs = None \<and> distinct (N ! i) \<and>
-    literals_are_in_\<L>\<^sub>i\<^sub>n (mset (N ! i)) \<and> \<not> tautology (mset (N ! i)) \<and> literals_are_in_\<L>\<^sub>i\<^sub>n_trail M \<and>
+  [\<lambda>((((((M, N), i), xs), clvls), lbd), outl). clvls = 0 \<and> i \<in># dom_m N \<and> xs = None \<and> distinct (N \<propto> i) \<and>
+    literals_are_in_\<L>\<^sub>i\<^sub>n (mset (N \<propto> i)) \<and> \<not> tautology (mset (N \<propto> i)) \<and> literals_are_in_\<L>\<^sub>i\<^sub>n_trail M \<and>
      no_dup M \<and> out_learned M None outl]\<^sub>a
   trail_assn\<^sup>k *\<^sub>a clauses_ll_assn\<^sup>k *\<^sub>a nat_assn\<^sup>k *\<^sub>a option_lookup_clause_assn\<^sup>d *\<^sub>a uint32_nat_assn\<^sup>k *\<^sub>a
       lbd_assn\<^sup>d *\<^sub>a out_learned_assn\<^sup>d \<rightarrow>
@@ -1099,18 +1100,18 @@ theorem resolve_lookup_conflict_merge_code_set_conflict[sepref_fr_rules]:
    (is \<open>?c \<in> [?pre]\<^sub>a ?im \<rightarrow> ?f\<close>)
 proof -
    have H: \<open>?c
-  \<in> [comp_PRE (\<langle>Id\<rangle>list_rel \<times>\<^sub>f \<langle>\<langle>Id\<rangle>list_rel\<rangle>list_rel \<times>\<^sub>f nat_rel \<times>\<^sub>f option_lookup_clause_rel \<times>\<^sub>f
+  \<in> [comp_PRE (\<langle>Id\<rangle>list_rel \<times>\<^sub>f Id \<times>\<^sub>f nat_rel \<times>\<^sub>f option_lookup_clause_rel \<times>\<^sub>f
         nat_rel \<times>\<^sub>f Id \<times>\<^sub>f Id)
-     (\<lambda>((((((M, N), i), xs), clvls), lbd), outl). i < length N \<and> xs = None \<and>
-         distinct (N ! i) \<and> literals_are_in_\<L>\<^sub>i\<^sub>n (mset (N ! i)) \<and> \<not> tautology (mset (N ! i)) \<and>
+     (\<lambda>((((((M, N), i), xs), clvls), lbd), outl). i \<in># dom_m N \<and> xs = None \<and>
+         distinct (N \<propto> i) \<and> literals_are_in_\<L>\<^sub>i\<^sub>n (mset (N \<propto> i)) \<and> \<not> tautology (mset (N \<propto> i)) \<and>
          clvls = 0 \<and> out_learned M None outl)
-     (\<lambda>_ ((((((M, N), i), _, xs), _), _), _). i < length N \<and> literals_are_in_\<L>\<^sub>i\<^sub>n_trail M \<and>
-         (\<forall>j<length (N ! i). atm_of (N ! i ! j) < length (snd xs)) \<and> no_dup M \<and>
-         literals_are_in_\<L>\<^sub>i\<^sub>n (mset (N ! i)) \<and> length (N ! i) \<le> uint_max)
+     (\<lambda>_ ((((((M, N), i), _, xs), _), _), _). i \<in># dom_m N \<and> literals_are_in_\<L>\<^sub>i\<^sub>n_trail M \<and>
+         (\<forall>j<length (N \<propto> i). atm_of (N \<propto> i ! j) < length (snd xs)) \<and> no_dup M \<and>
+         literals_are_in_\<L>\<^sub>i\<^sub>n (mset (N \<propto> i)) \<and> length (N \<propto> i) \<le> uint_max)
      (\<lambda>_. True)]\<^sub>a
    hrp_comp ((hr_comp trail_pol_assn trail_pol)\<^sup>k *\<^sub>a clauses_ll_assn\<^sup>k *\<^sub>a nat_assn\<^sup>k *\<^sub>a
        conflict_option_rel_assn\<^sup>d *\<^sub>a uint32_nat_assn\<^sup>k *\<^sub>a lbd_assn\<^sup>d *\<^sub>a out_learned_assn\<^sup>d)
-     (\<langle>Id\<rangle>list_rel \<times>\<^sub>f \<langle>\<langle>Id\<rangle>list_rel\<rangle>list_rel \<times>\<^sub>f nat_rel \<times>\<^sub>f option_lookup_clause_rel \<times>\<^sub>f
+     (\<langle>Id\<rangle>list_rel \<times>\<^sub>f Id \<times>\<^sub>f nat_rel \<times>\<^sub>f option_lookup_clause_rel \<times>\<^sub>f
          nat_rel \<times>\<^sub>f Id \<times>\<^sub>f Id) \<rightarrow>
     hr_comp (conflict_option_rel_assn *a uint32_nat_assn *a lbd_assn *a out_learned_assn)
       (option_lookup_clause_rel \<times>\<^sub>f (nat_rel \<times>\<^sub>f (Id \<times>\<^sub>f Id)))\<close> (is \<open>_ \<in> [?pre']\<^sub>a ?im' \<rightarrow> ?f'\<close>)
@@ -1141,12 +1142,12 @@ qed
 
 lemma resolve_lookup_conflict_aa_merge_conflict_m:
   \<open>(uncurry6 resolve_lookup_conflict_aa, uncurry6 merge_conflict_m) \<in>
-    [\<lambda>((((((M, N), i), xs), clvls), lbd), out). i < length N \<and> xs \<noteq> None \<and> distinct (N ! i) \<and>
-       literals_are_in_\<L>\<^sub>i\<^sub>n (mset (N ! i)) \<and> \<not>tautology (mset (N ! i)) \<and>
-       (\<forall>L \<in> set (tl (N ! i)). - L \<notin># the xs) \<and>
+    [\<lambda>((((((M, N), i), xs), clvls), lbd), out). i \<in># dom_m N \<and> xs \<noteq> None \<and> distinct (N \<propto> i) \<and>
+       literals_are_in_\<L>\<^sub>i\<^sub>n (mset (N \<propto> i)) \<and> \<not>tautology (mset (N \<propto> i)) \<and>
+       (\<forall>L \<in> set (tl (N \<propto> i)). - L \<notin># the xs) \<and>
        literals_are_in_\<L>\<^sub>i\<^sub>n (the xs) \<and> clvls = card_max_lvl M (the xs) \<and>
        out_learned M xs out]\<^sub>f
-    \<langle>Id\<rangle>list_rel \<times>\<^sub>f \<langle>\<langle>Id\<rangle>list_rel\<rangle>list_rel \<times>\<^sub>f nat_rel \<times>\<^sub>f option_lookup_clause_rel \<times>\<^sub>f nat_rel \<times>\<^sub>f Id
+    \<langle>Id\<rangle>list_rel \<times>\<^sub>f Id \<times>\<^sub>f nat_rel \<times>\<^sub>f option_lookup_clause_rel \<times>\<^sub>f nat_rel \<times>\<^sub>f Id
          \<times>\<^sub>f Id \<rightarrow>
     \<langle>option_lookup_clause_rel \<times>\<^sub>r nat_rel \<times>\<^sub>r Id \<times>\<^sub>r Id\<rangle>nres_rel\<close>
 proof -
@@ -1154,17 +1155,17 @@ proof -
     \<le> \<Down> (option_lookup_clause_rel \<times>\<^sub>r Id)
        (merge_conflict_m M N i (Some D) clvls lbd outl)\<close>
     if
-      \<open>i < length N\<close> and
+      \<open>i \<in># dom_m N\<close> and
       ocr: \<open>((b, n, xs), Some D) \<in> option_lookup_clause_rel\<close> and
-      dist: \<open>distinct (N ! i)\<close> and
-      lits: \<open>literals_are_in_\<L>\<^sub>i\<^sub>n (mset (N ! i))\<close> and
-      tauto: \<open>\<not>tautology (mset (N ! i))\<close> and
-      \<open>\<forall>L \<in> set (tl (N ! i)). - L \<notin># D\<close> and
+      dist: \<open>distinct (N \<propto> i)\<close> and
+      lits: \<open>literals_are_in_\<L>\<^sub>i\<^sub>n (mset (N \<propto> i))\<close> and
+      tauto: \<open>\<not>tautology (mset (N \<propto> i))\<close> and
+      \<open>\<forall>L \<in> set (tl (N \<propto> i)). - L \<notin># D\<close> and
       lits_D: \<open>literals_are_in_\<L>\<^sub>i\<^sub>n D\<close> and
       clvls: \<open>clvls = card_max_lvl M D\<close> and
       out: \<open>out_learned M (Some D) outl\<close>
     for b n xs N i M clvls lbd D outl
-    using lookup_conflict_merge'_spec[of b n xs D \<open>N!i\<close> clvls M 1 outl lbd] that dist lits_D clvls
+    using lookup_conflict_merge'_spec[of b n xs D \<open>N\<propto>i\<close> clvls M 1 outl lbd] that dist lits_D clvls
       out
     unfolding merge_conflict_m_g_def tl_drop_def[symmetric] resolve_lookup_conflict_aa_def
       merge_conflict_m_def
@@ -1176,30 +1177,30 @@ qed
 
 theorem resolve_lookup_conflict_merge_code_merge_conflict_m[sepref_fr_rules]:
   \<open>(uncurry6 resolve_lookup_conflict_merge_code, uncurry6 merge_conflict_m) \<in>
-  [\<lambda>((((((M, N), i), xs), clvls), lbd), outl). clvls = card_max_lvl M (the xs) \<and> i < length N \<and>
-      xs \<noteq> None \<and> distinct (N ! i) \<and> \<not>tautology (the xs) \<and>
-     literals_are_in_\<L>\<^sub>i\<^sub>n (mset (N ! i)) \<and> \<not> tautology (mset (N ! i)) \<and> literals_are_in_\<L>\<^sub>i\<^sub>n_trail M \<and>
+  [\<lambda>((((((M, N), i), xs), clvls), lbd), outl). clvls = card_max_lvl M (the xs) \<and> i \<in># dom_m N \<and>
+      xs \<noteq> None \<and> distinct (N \<propto> i) \<and> \<not>tautology (the xs) \<and>
+     literals_are_in_\<L>\<^sub>i\<^sub>n (mset (N \<propto> i)) \<and> \<not> tautology (mset (N \<propto> i)) \<and> literals_are_in_\<L>\<^sub>i\<^sub>n_trail M \<and>
      no_dup M \<and> literals_are_in_\<L>\<^sub>i\<^sub>n (the xs) \<and>
-     (\<forall>L \<in> set (tl (N ! i)). - L \<notin># the xs) \<and> out_learned M xs outl]\<^sub>a
+     (\<forall>L \<in> set (tl (N \<propto> i)). - L \<notin># the xs) \<and> out_learned M xs outl]\<^sub>a
   trail_assn\<^sup>k *\<^sub>a clauses_ll_assn\<^sup>k *\<^sub>a nat_assn\<^sup>k *\<^sub>a option_lookup_clause_assn\<^sup>d *\<^sub>a uint32_nat_assn\<^sup>k *\<^sub>a
       lbd_assn\<^sup>d *\<^sub>a out_learned_assn\<^sup>d \<rightarrow>
     option_lookup_clause_assn *a uint32_nat_assn *a lbd_assn *a out_learned_assn\<close>
    (is \<open>?c \<in> [?pre]\<^sub>a ?im \<rightarrow> ?f\<close>)
 proof -
    have H: \<open>?c
-  \<in> [comp_PRE (\<langle>Id\<rangle>list_rel \<times>\<^sub>f \<langle>\<langle>Id\<rangle>list_rel\<rangle>list_rel \<times>\<^sub>f nat_rel \<times>\<^sub>f option_lookup_clause_rel \<times>\<^sub>f
+  \<in> [comp_PRE (\<langle>Id\<rangle>list_rel \<times>\<^sub>f Id \<times>\<^sub>f nat_rel \<times>\<^sub>f option_lookup_clause_rel \<times>\<^sub>f
       nat_rel \<times>\<^sub>f Id \<times>\<^sub>f Id)
-     (\<lambda>((((((M, N), i), xs), clvls), lbd), out). i < length N \<and> xs \<noteq> None \<and> distinct (N ! i) \<and>
-         literals_are_in_\<L>\<^sub>i\<^sub>n (mset (N ! i)) \<and> \<not> tautology (mset (N ! i)) \<and>
-         (\<forall>L\<in>set (tl (N ! i)). - L \<notin># the xs) \<and> literals_are_in_\<L>\<^sub>i\<^sub>n (the xs) \<and>
+     (\<lambda>((((((M, N), i), xs), clvls), lbd), out). i \<in># dom_m N \<and> xs \<noteq> None \<and> distinct (N \<propto> i) \<and>
+         literals_are_in_\<L>\<^sub>i\<^sub>n (mset (N \<propto> i)) \<and> \<not> tautology (mset (N \<propto> i)) \<and>
+         (\<forall>L\<in>set (tl (N \<propto> i)). - L \<notin># the xs) \<and> literals_are_in_\<L>\<^sub>i\<^sub>n (the xs) \<and>
          clvls = card_max_lvl M (the xs) \<and> out_learned M xs out)
-     (\<lambda>_ ((((((M, N), i), _, xs), _), _), out). i < length N \<and> literals_are_in_\<L>\<^sub>i\<^sub>n_trail M \<and>
-         (\<forall>j<length (N ! i). atm_of (N ! i ! j) < length (snd xs)) \<and> no_dup M \<and>
-         literals_are_in_\<L>\<^sub>i\<^sub>n (mset (N ! i)) \<and> length (N ! i) \<le> uint_max)
+     (\<lambda>_ ((((((M, N), i), _, xs), _), _), out). i \<in># dom_m N \<and> literals_are_in_\<L>\<^sub>i\<^sub>n_trail M \<and>
+         (\<forall>j<length (N \<propto> i). atm_of (N \<propto> i ! j) < length (snd xs)) \<and> no_dup M \<and>
+         literals_are_in_\<L>\<^sub>i\<^sub>n (mset (N \<propto> i)) \<and> length (N \<propto> i) \<le> uint_max)
      (\<lambda>_. True)]\<^sub>a
    hrp_comp ((hr_comp trail_pol_assn trail_pol)\<^sup>k *\<^sub>a clauses_ll_assn\<^sup>k *\<^sub>a nat_assn\<^sup>k *\<^sub>a
                conflict_option_rel_assn\<^sup>d *\<^sub>a uint32_nat_assn\<^sup>k *\<^sub>a lbd_assn\<^sup>d *\<^sub>a out_learned_assn\<^sup>d)
-      (\<langle>Id\<rangle>list_rel \<times>\<^sub>f \<langle>\<langle>Id\<rangle>list_rel\<rangle>list_rel \<times>\<^sub>f nat_rel \<times>\<^sub>f option_lookup_clause_rel \<times>\<^sub>f nat_rel \<times>\<^sub>f
+      (\<langle>Id\<rangle>list_rel \<times>\<^sub>f Id \<times>\<^sub>f nat_rel \<times>\<^sub>f option_lookup_clause_rel \<times>\<^sub>f nat_rel \<times>\<^sub>f
                       Id \<times>\<^sub>f Id) \<rightarrow>
    hr_comp (conflict_option_rel_assn *a uint32_nat_assn *a lbd_assn *a out_learned_assn)
       (option_lookup_clause_rel \<times>\<^sub>f (nat_rel \<times>\<^sub>f (Id \<times>\<^sub>f Id)))\<close> (is \<open>_ \<in> [?pre']\<^sub>a ?im' \<rightarrow> ?f'\<close>)
@@ -1581,8 +1582,8 @@ where
         (\<lambda>(cach, analyse, b). analyse \<noteq> [])
         (\<lambda>(cach, analyse, b). do {
             ASSERT(analyse \<noteq> []);
-            ASSERT(fst (last analyse) < length NU);
-            let C = NU ! fst (last analyse);
+            ASSERT(fst (last analyse) \<in># dom_m NU);
+            let C = NU \<propto> fst (last analyse);
             ASSERT(length C > 0); (* \<ge> 2 ? *)
             let i = snd (last analyse);
             ASSERT(C!0 \<in> lits_of_l M);
@@ -1626,9 +1627,9 @@ lemma lit_redundant_rec_wl_lookup_mark_failed_lits_stack_inv:
     \<open>x' = (x1, x2)\<close> and
     \<open>x2b = (x1c, x2c)\<close> and
     \<open>x = (x1b, x2b)\<close> and
-    \<open>NU ! fst (last x1a) ! 0 \<in> lits_of_l M\<close> and
-    \<open>\<not> length (NU ! fst (last x1a)) \<le> snd (last x1a)\<close> and
-    \<open>get_literal_and_remove_of_analyse_wl (NU ! fst (last x1c)) x1c = (x1e, x2e)\<close>
+    \<open>NU \<propto> fst (last x1a) ! 0 \<in> lits_of_l M\<close> and
+    \<open>\<not> length (NU \<propto> fst (last x1a)) \<le> snd (last x1a)\<close> and
+    \<open>get_literal_and_remove_of_analyse_wl (NU \<propto> fst (last x1c)) x1c = (x1e, x2e)\<close>
   shows \<open>mark_failed_lits_stack_inv NU x2e x1b\<close>
 proof -
   show ?thesis
@@ -1858,18 +1859,21 @@ context isasat_input_bounded
 begin
 
 lemma minimize_and_extract_highest_lookup_conflict_iterate_over_conflict:
-  fixes D :: \<open>nat clause\<close> and s and s' and NU :: \<open>nat clauses_l\<close> and S :: \<open>nat twl_st_wl\<close>
-  defines
-    \<open>S' \<equiv> st_l_of_wl None S\<close> and
-    \<open>S'' \<equiv> twl_st_of_wl None S\<close> and
-    \<open>S''' \<equiv> state\<^sub>W_of (twl_st_of_wl None S)\<close>
+  fixes D :: \<open>nat clause\<close> and S' :: \<open>nat twl_st_l\<close> and NU :: \<open>nat clauses_l\<close> and S :: \<open>nat twl_st_wl\<close>
+     and S'' :: \<open>nat twl_st\<close>
+   defines
+ (*   \<open>S' \<equiv> st_l_of_wl None S\<close> and
+    \<open>S'' \<equiv> twl_st_of_wl None S\<close> and *)
+    \<open>S''' \<equiv> state\<^sub>W_of S''\<close>
   defines
     \<open>M \<equiv> get_trail_wl S\<close> and
     NU: \<open>NU \<equiv> get_clauses_wl S\<close> and
-    NU'_def: \<open>NU' \<equiv> mset `# mset (tl NU)\<close> and
+    NU'_def: \<open>NU' \<equiv> mset `# ran_mf NU\<close> and
     NUE: \<open>NUE \<equiv> get_unit_learned S + get_unit_init_clss S\<close> and
     M': \<open>M' \<equiv> trail S'''\<close>
   assumes
+    S_S': \<open>(S, S') \<in> state_wl_l None\<close> and
+    S'_S'': \<open>(S', S'') \<in> twl_st_l None\<close> and
     D'_D: \<open>mset (tl outl) = D\<close> and
     M_D: \<open>M \<Turnstile>as CNot D\<close> and
     dist_D: \<open>distinct_mset D\<close> and
@@ -1891,19 +1895,20 @@ lemma minimize_and_extract_highest_lookup_conflict_iterate_over_conflict:
 proof -
   let ?UE = \<open>get_unit_learned S\<close>
   let ?NE = \<open>get_unit_init_clss S\<close>
-  define u where \<open>u = get_learned_wl S\<close>
   define N U where
-    \<open>N \<equiv> mset `# mset (take u (tl NU))\<close> and
-    \<open>U \<equiv> mset `# mset (drop u (tl NU))\<close>
+    \<open>N \<equiv> mset `# init_clss_lf NU\<close> and
+    \<open>U \<equiv> mset `# learned_clss_lf NU\<close>
   obtain E where
      S''': \<open>S''' = (M', N + ?NE, U + ?UE, E)\<close>
-    using M' unfolding S''_def S'''_def N_def U_def u_def NU
-    by (cases S) (auto simp: get_unit_init_clss_def get_unit_learned_def drop_Suc
+    using M' S_S' S'_S'' unfolding S'''_def N_def U_def NU
+    by (cases S) (auto simp: state_wl_l_def twl_st_l_def
         mset_take_mset_drop_mset')
-  then have NU_N_U: \<open>mset `# mset (tl NU) = N + U\<close>
-    unfolding NU unfolding S''_def S'''_def
-    by (cases S) (auto simp: get_unit_init_clss_def get_unit_learned_def
-        mset_take_mset_drop_mset')
+  then have NU_N_U: \<open>mset `# ran_mf NU = N + U\<close>
+    using NU S_S' S'_S'' unfolding S'''_def N_def U_def
+    apply (subst all_clss_l_ran_m[symmetric])
+    apply (subst image_mset_union[symmetric])
+    apply (subst image_mset_union[symmetric])
+    by (auto simp: mset_take_mset_drop_mset')
   let ?NU = \<open>N + ?NE + U + ?UE\<close>
   have NU'_N_U: \<open>NU' = N + U\<close>
     unfolding NU'_def N_def U_def mset_append[symmetric] image_mset_union[symmetric]
@@ -1912,13 +1917,13 @@ proof -
     unfolding NUE NU'_N_U by (auto simp: ac_simps)
   have struct_inv_S''': \<open>cdcl\<^sub>W_restart_mset.cdcl\<^sub>W_all_struct_inv (M', N + get_unit_init_clss S,
           U + get_unit_learned S, E)\<close>
-    using struct_invs unfolding twl_struct_invs_def S''_def S'''_def[symmetric] S'''
+    using struct_invs unfolding twl_struct_invs_def S'''_def[symmetric] S'''
     by fast
   then have n_d: \<open>no_dup M'\<close>
     unfolding cdcl\<^sub>W_restart_mset.cdcl\<^sub>W_all_struct_inv_def cdcl\<^sub>W_restart_mset.cdcl\<^sub>W_M_level_inv_def
       trail.simps by fast
   then have n_d: \<open>no_dup M\<close>
-    unfolding M_def M' S'''_def by (cases S) auto
+    using S_S' S'_S'' unfolding M_def M' S'''_def by (auto simp: twl_st_wl twl_st_l twl_st)
 
   define R where
     \<open>R = {((D':: nat clause, i, cach :: nat \<Rightarrow> minimize_status, outl' :: out_learned),
@@ -2019,7 +2024,7 @@ proof -
     have M_x1: \<open>M \<Turnstile>as CNot E\<close>
       by (metis CNot_plus M_D \<open>E \<subseteq># D\<close> subset_mset.le_iff_add true_annots_union)
     then have M'_x1: \<open>M' \<Turnstile>as CNot E\<close>
-      unfolding M' M_def S'''_def by (cases S) auto
+      using S_S' S'_S'' unfolding M' M_def S'''_def by (auto simp: twl_st)
     have \<open>outl' ! x1d \<in># E\<close>
       using \<open>E = mset (tl outl')\<close> \<open>x1d < length outl'\<close> \<open>0 < x1d\<close>
       by (auto simp: nth_in_set_tl)
@@ -2027,8 +2032,7 @@ proof -
     have 1:
     \<open>literal_redundant_wl_lookup M NU nxs cach ?L lbd \<le> \<Down> Id (literal_redundant_wl M NU nxs cach ?L lbd)\<close>
       by (rule literal_redundant_wl_lookup_literal_redundant_wl)
-        (use n_d lits M_x1 struct_invs add_inv \<open>outl' ! x1d \<in># E\<close> \<open>E = nxs\<close> in
-          \<open>auto simp: S'_def S''_def\<close>)
+        (use n_d lits M_x1 struct_invs add_inv \<open>outl' ! x1d \<in># E\<close> \<open>E = nxs\<close> in auto)
     then have 1:
     \<open>literal_redundant_wl_lookup M NU nxs cach ?L lbd \<le> (literal_redundant_wl M NU nxs cach ?L lbd)\<close>
       by simp
@@ -2036,12 +2040,12 @@ proof -
     have 2:
     \<open>literal_redundant_wl M NU nxs cach ?L lbd \<le> \<Down>
        (Id \<times>\<^sub>r {(analyse, analyse'). analyse' = convert_analysis_list NU analyse \<and>
-          (\<forall>(i, j)\<in> set analyse. j \<le> length (NU!i) \<and> i < length NU \<and> j \<ge> 1 \<and> i > 0)} \<times>\<^sub>r bool_rel)
+          (\<forall>(i, j)\<in> set analyse. j \<le> length (NU\<propto>i) \<and> i \<in># dom_m NU \<and> j \<ge> 1 \<and> i > 0)} \<times>\<^sub>r bool_rel)
        (literal_redundant M' NU' nxs cach ?L)\<close>
-      by (rule literal_redundant_wl_literal_redundant[of S,
+      by (rule literal_redundant_wl_literal_redundant[of S S' S'',
             unfolded M_def[symmetric] NU[symmetric] M'[symmetric] S'''_def[symmetric]
             NU'_def[symmetric]])
-         (use M_x1 struct_invs add_inv \<open>outl' ! x1d \<in># E\<close> \<open>E = nxs\<close> in \<open>auto simp: S'_def S''_def\<close>)
+         (use S_S' S'_S'' M_x1 struct_invs add_inv \<open>outl' ! x1d \<in># E\<close> \<open>E = nxs\<close> in auto)
 
     have 3:
        \<open>literal_redundant M' (N + U) nxs cach ?L \<le>
@@ -2273,14 +2277,14 @@ begin
 private lemma mark_failed_lits_stack_inv_helper1: \<open>mark_failed_lits_stack_inv a ba a2' \<Longrightarrow>
        a1' < length ba \<Longrightarrow>
        (a1'a, a2'a) = ba ! a1' \<Longrightarrow>
-       a1'a < length a\<close>
+       a1'a \<in># dom_m a\<close>
   using nth_mem[of a1' ba] unfolding  mark_failed_lits_stack_inv_def
   by (auto simp del: nth_mem)
 
 private lemma mark_failed_lits_stack_inv_helper2: \<open>mark_failed_lits_stack_inv a ba a2' \<Longrightarrow>
        a1' < length ba \<Longrightarrow>
        (a1'a, a2'a) = ba ! a1' \<Longrightarrow>
-       a2'a - Suc 0 < length (a ! a1'a)\<close>
+       a2'a - Suc 0 < length (a \<propto> a1'a)\<close>
   using nth_mem[of a1' ba] unfolding  mark_failed_lits_stack_inv_def
   by (auto simp del: nth_mem)
 
@@ -2290,11 +2294,13 @@ sepref_thm mark_failed_lits_stack_code
       cach_refinement_assn\<close>
   supply [[goals_limit = 1]] neq_Nil_revE[elim!] image_image[simp] length_rll_def[simp]
     mark_failed_lits_stack_inv_helper1[dest] mark_failed_lits_stack_inv_helper2[dest]
+    fmap_length_rll_u_def[simp]
   unfolding mark_failed_lits_stack_def
     conflict_min_cach_set_failed_def[symmetric]
     conflict_min_cach_def[symmetric]
     get_literal_and_remove_of_analyse_wl_def
     nth_rll_def[symmetric]
+    fmap_rll_def[symmetric]
   by sepref
 
 end
@@ -2311,7 +2317,7 @@ lemmas mark_failed_lits_stack_code_hnr =
 
 lemma mark_failed_lits_wl_hnr[sepref_fr_rules]:
   \<open>(uncurry2 mark_failed_lits_stack_code, uncurry2 mark_failed_lits_wl)
-     \<in> [\<lambda>((a, b), ba). literals_are_in_\<L>\<^sub>i\<^sub>n_mm (mset `# mset (tl a)) \<and>
+     \<in> [\<lambda>((a, b), ba). literals_are_in_\<L>\<^sub>i\<^sub>n_mm ((mset \<circ> fst) `# ran_m a) \<and>
          mark_failed_lits_stack_inv a b ba]\<^sub>a
         clauses_ll_assn\<^sup>k *\<^sub>a analyse_refinement_assn\<^sup>d *\<^sub>a cach_refinement_assn\<^sup>d \<rightarrow>
         cach_refinement_assn\<close>
@@ -2332,12 +2338,12 @@ lemma literals_are_in_\<L>\<^sub>i\<^sub>n_trail_uminus_in_lits_of_l_atms:
   using literals_are_in_\<L>\<^sub>i\<^sub>n_trail_uminus_in_lits_of_l[of M a]
   unfolding in_\<L>\<^sub>a\<^sub>l\<^sub>l_atm_of_in_atms_of_iff[symmetric] atms_of_\<L>\<^sub>a\<^sub>l\<^sub>l_\<A>\<^sub>i\<^sub>n[symmetric]
   .
-
+(* TODO fst (lst last) \<le> uint_max? *)
 sepref_register lit_redundant_rec_wl_lookup
 sepref_thm lit_redundant_rec_wl_lookup_code
   is \<open>uncurry5 (PR_CONST lit_redundant_rec_wl_lookup)\<close>
   :: \<open>[\<lambda>(((((M, NU), D), cach), analysis), lbd).
-         literals_are_in_\<L>\<^sub>i\<^sub>n_mm (mset `# mset (tl NU)) \<and>
+         literals_are_in_\<L>\<^sub>i\<^sub>n_mm (mset `# ran_mf NU) \<and>
          literals_are_in_\<L>\<^sub>i\<^sub>n_trail M]\<^sub>a
       trail_assn\<^sup>k *\<^sub>a clauses_ll_assn\<^sup>k *\<^sub>a lookup_clause_assn\<^sup>k *\<^sub>a
         cach_refinement_assn\<^sup>d *\<^sub>a analyse_refinement_assn\<^sup>d *\<^sub>a lbd_assn\<^sup>k \<rightarrow>
@@ -2346,15 +2352,21 @@ sepref_thm lit_redundant_rec_wl_lookup_code
     literals_are_in_\<L>\<^sub>i\<^sub>n_trail_uminus_in_lits_of_l[intro]
     literals_are_in_\<L>\<^sub>i\<^sub>n_trail_in_lits_of_l_atms[intro] length_rll_def[simp]
     literals_are_in_\<L>\<^sub>i\<^sub>n_trail_uminus_in_lits_of_l_atms[intro] nth_rll_def[simp]
+    fmap_length_rll_u_def[simp]
+    fmap_length_rll_def[simp]
   unfolding lit_redundant_rec_wl_lookup_def
     conflict_min_cach_set_removable_def[symmetric]
     conflict_min_cach_def[symmetric]
     get_literal_and_remove_of_analyse_wl_def
     nth_rll_def[symmetric] PR_CONST_def
+    fmap_rll_u_def[symmetric]
+    fmap_rll_def[symmetric]
   apply (rewrite at \<open>(_, \<hole>, _)\<close> arl.fold_custom_empty)+
   apply (rewrite at \<open>op_arl_empty\<close> annotate_assn[where A=analyse_refinement_assn])
-  apply (rewrite at \<open>let _ = _ ! _ in _\<close> Let_def)
+  apply (rewrite at \<open>let _ = _ \<propto> _ in _\<close> Let_def)
   unfolding nth_rll_def[symmetric] length_rll_def[symmetric]
+    fmap_rll_def[symmetric]
+    fmap_length_rll_def[symmetric]
   by sepref (* slow *)
 
 concrete_definition (in -) lit_redundant_rec_wl_lookup_code
@@ -2427,18 +2439,21 @@ context isasat_input_bounded
 begin
 
 lemma
-  fixes D :: \<open>nat clause\<close> and s and s' and NU :: \<open>nat clauses_l\<close> and S :: \<open>nat twl_st_wl\<close>
+  fixes D :: \<open>nat clause\<close> and s and s' and NU :: \<open>nat clauses_l\<close> and
+    S :: \<open>nat twl_st_wl\<close> and S' :: \<open>nat twl_st_l\<close> and S'' :: \<open>nat twl_st\<close>
   defines
-    \<open>S' \<equiv> st_l_of_wl None S\<close> and
-    \<open>S'' \<equiv> twl_st_of_wl None S\<close> and
-    \<open>S''' \<equiv> state\<^sub>W_of (twl_st_of_wl None S)\<close>
+(*     \<open>S' \<equiv> st_l_of_wl None S\<close> and
+    \<open>S'' \<equiv> twl_st_of_wl None S\<close> and *)
+    \<open>S''' \<equiv> state\<^sub>W_of S''\<close>
   defines
     \<open>M \<equiv> get_trail_wl S\<close> and
     NU: \<open>NU \<equiv> get_clauses_wl S\<close> and
-    NU'_def: \<open>NU' \<equiv> mset `# mset (tl NU)\<close> and
+    NU'_def: \<open>NU' \<equiv> mset `# ran_mf NU\<close> and
     NUE: \<open>NUE \<equiv> get_unit_learned S + get_unit_init_clss S\<close> and
     M': \<open>M' \<equiv> trail S'''\<close>
   assumes
+    S_S': \<open>(S, S') \<in> state_wl_l None\<close> and
+    S'_S'': \<open>(S', S'') \<in> twl_st_l None\<close> and
     D'_D: \<open>mset (tl outl) = D\<close> and
     M_D: \<open>M \<Turnstile>as CNot D\<close> and
     dist_D: \<open>distinct_mset D\<close> and
@@ -2460,7 +2475,7 @@ proof -
   show ?thesis
     apply (rule order.trans)
      apply (rule minimize_and_extract_highest_lookup_conflict_iterate_over_conflict[OF
-          assms(9-20)[unfolded assms(1-8)],
+          assms(7-20)[unfolded assms(1-8)],
           unfolded assms(1-8)[symmetric]])
     apply (rule order.trans)
      apply (rule conc_fun_mono[OF iterate_over_conflict_spec[OF NU_P_D dist_D]])
@@ -2477,24 +2492,6 @@ sepref_definition (in -) confl_find_next_index_code
   by sepref
 
 declare (in -) confl_find_next_index_code.refine[sepref_fr_rules]
-
-(* TODO Move + setup for efficient array accesses *)
-definition arl_set'_u where
-  \<open>arl_set'_u a i x = arl_set a (nat_of_uint32 i) x\<close>
-
-definition arl_set_u :: \<open>'a::heap array_list \<Rightarrow> uint32 \<Rightarrow> 'a \<Rightarrow> 'a array_list Heap\<close>where
-  \<open>arl_set_u a i x = arl_set'_u a i x\<close>
-
-lemma arl_set_hnr_u[sepref_fr_rules]:
-  \<open>CONSTRAINT is_pure A \<Longrightarrow>
-    (uncurry2 arl_set_u, uncurry2 (RETURN \<circ>\<circ>\<circ> op_list_set)) \<in>
-     [pre_list_set]\<^sub>a (arl_assn A)\<^sup>d *\<^sub>a uint32_nat_assn\<^sup>k *\<^sub>a A\<^sup>k \<rightarrow> arl_assn A\<close>
-  by sepref_to_hoare
-    (sep_auto simp: uint32_nat_rel_def br_def ex_assn_up_eq2 array_assn_def is_array_def
-      hr_comp_def list_rel_pres_length list_rel_update heap_array_set'_u_def
-      heap_array_set_u_def Array.upd'_def arl_set_u_def arl_set'_u_def arl_assn_def
-     nat_of_uint32_code[symmetric])
-(* End Move *)
 
 
 sepref_definition delete_index_and_swap_code
@@ -2571,7 +2568,7 @@ sepref_register literal_redundant_wl_lookup
 sepref_thm literal_redundant_wl_lookup_code
   is \<open>uncurry5 (PR_CONST literal_redundant_wl_lookup)\<close>
   :: \<open>[\<lambda>(((((M, NU), D), cach), L), lbd). literals_are_in_\<L>\<^sub>i\<^sub>n_trail M \<and>
-        literals_are_in_\<L>\<^sub>i\<^sub>n_mm (mset `# mset (tl NU))]\<^sub>a
+        literals_are_in_\<L>\<^sub>i\<^sub>n_mm (mset `# ran_mf NU)]\<^sub>a
       trail_assn\<^sup>k *\<^sub>a clauses_ll_assn\<^sup>k *\<^sub>a lookup_clause_assn\<^sup>k *\<^sub>a
       cach_refinement_assn\<^sup>d *\<^sub>a unat_lit_assn\<^sup>k *\<^sub>a lbd_assn\<^sup>k \<rightarrow>
       cach_refinement_assn *a analyse_refinement_assn *a bool_assn\<close>
@@ -2603,7 +2600,7 @@ sepref_register minimize_and_extract_highest_lookup_conflict
 sepref_thm minimize_and_extract_highest_lookup_conflict_code
   is \<open>uncurry5 (PR_CONST minimize_and_extract_highest_lookup_conflict)\<close>
   :: \<open>[\<lambda>(((((M, NU), D), cach), lbd), outl). literals_are_in_\<L>\<^sub>i\<^sub>n_trail M \<and>
-        literals_are_in_\<L>\<^sub>i\<^sub>n_mm (mset `# mset (tl NU))]\<^sub>a
+        literals_are_in_\<L>\<^sub>i\<^sub>n_mm (mset `# ran_mf NU)]\<^sub>a
        trail_assn\<^sup>k *\<^sub>a clauses_ll_assn\<^sup>k *\<^sub>a lookup_clause_assn\<^sup>d *\<^sub>a
         cach_refinement_assn\<^sup>d *\<^sub>a lbd_assn\<^sup>k *\<^sub>a out_learned_assn\<^sup>d \<rightarrow>
       lookup_clause_assn *a cach_refinement_assn *a out_learned_assn\<close>
