Weidenbach_Book/WB_More_Refinement.thy
@@ -284,6 +284,9 @@ lemma RES_RETURN_RES3:
 lemma bind_refine_res: \<open>(\<And>x. x \<in> \<Phi> \<Longrightarrow> f x \<le> \<Down> R M) \<Longrightarrow> M' \<le> RES \<Phi> \<Longrightarrow> M' \<bind> f \<le> \<Down> R M\<close>
   by (auto simp add: pw_le_iff refine_pw_simps)
 
+thm ref_WHILEI_invarI WHILEI_le_rule
+thm WHILEI_invisible_refine_genR
+
 text \<open>
   This theorem adds the invariant at the beginning of next iteration to the current invariant,
   i.e., the invariant is added as a post-condition on the current iteration.
