Weidenbach_Book/Watched_Literals_Watch_List_Domain.thy
@@ -288,17 +288,18 @@ lemma uminus_\<A>\<^sub>i\<^sub>n_iff: \<open>- L \<in># \<L>\<^sub>a\<^sub>l\<^
 definition literals_are_in_\<L>\<^sub>i\<^sub>n_mm :: \<open>nat clauses \<Rightarrow> bool\<close> where
   \<open>literals_are_in_\<L>\<^sub>i\<^sub>n_mm C \<longleftrightarrow> set_mset (all_lits_of_mm C) \<subseteq> set_mset \<L>\<^sub>a\<^sub>l\<^sub>l\<close>
 
+(*TODO Move to replace literals_are_in_\<L>\<^sub>i\<^sub>n_mm_in_\<L>\<^sub>a\<^sub>l\<^sub>l*)
 lemma literals_are_in_\<L>\<^sub>i\<^sub>n_mm_in_\<L>\<^sub>a\<^sub>l\<^sub>l:
   assumes
-    N1: \<open>literals_are_in_\<L>\<^sub>i\<^sub>n_mm (mset `# mset xs)\<close> and
-    i_xs: \<open>i < length xs\<close> and j_xs: \<open>j < length (xs ! i)\<close>
-  shows \<open>xs ! i ! j \<in># \<L>\<^sub>a\<^sub>l\<^sub>l\<close>
+    N1: \<open>literals_are_in_\<L>\<^sub>i\<^sub>n_mm (mset `# ran_mf xs)\<close> and
+    i_xs: \<open>i \<in># dom_m xs\<close> and j_xs: \<open>j < length (xs \<propto> i)\<close>
+  shows \<open>xs \<propto> i ! j \<in># \<L>\<^sub>a\<^sub>l\<^sub>l\<close>
 proof -
-  have \<open>xs ! i \<in># mset xs\<close>
+  have \<open>xs \<propto> i \<in># ran_mf xs\<close>
     using i_xs by auto
-  then have \<open>xs ! i ! j \<in> set_mset (all_lits_of_mm (mset `# mset xs))\<close>
+  then have \<open>xs \<propto> i ! j \<in> set_mset (all_lits_of_mm (mset `# ran_mf xs))\<close>
     using j_xs by (auto simp: in_all_lits_of_mm_ain_atms_of_iff atms_of_ms_def Bex_def
-      intro!: exI[of _ \<open>xs ! i\<close>])
+      intro!: exI[of _ \<open>xs \<propto> i\<close>])
   then show ?thesis
     using N1 unfolding literals_are_in_\<L>\<^sub>i\<^sub>n_mm_def by blast
 qed
